\documentclass{report}

\usepackage[T2A]{fontenc}
\usepackage[russian]{babel}
\usepackage{graphicx}
\usepackage{float}
\usepackage{hyperref}
\usepackage{amsmath}
\usepackage{diffcoeff,amssymb}
\usepackage{mathtools}
\usepackage{eturch}

\input{preamble}
\input{macros}
\input{letterfonts}


\title{\Huge{Матан}\\ Решение дз №4}
\author{\huge{Евгений Турчанин}}
\date{}

\begin{document}
\maketitle

\qs{}{
\begin{enumerate}
	\item $\lim\limits_{n\to\infty} \Bigl(\dfrac{n^2}{n+1}-\dfrac{n^3}{n^2+1}\Bigr)$
	\item $\lim\limits_{n\to\infty} \dfrac{(n+1)^4-(n-1)^4}{(n+1)^3+(n-1)^3}$
	\item $\lim\limits_{n\to\infty} \bigl(\sqrt[\leftroot{0}\uproot{2}3]{n^3+2n^2+1}-n \bigr)$
	\item $\lim\limits_{n\to\infty} \dfrac{\sqrt{n^2+1}-\sqrt{n^2-1}}{\sqrt{n^2+1}-n-1}$
	\item $\lim\limits_{n\to\infty} \displaystyle \sum_{k=1}^n \dfrac{1}{k(k+1)}$
\end{enumerate}
}

\begin{enumerate}
\item $\lim\limits_{n\to\infty} \left(\dfrac{n^2}{n+1}-\dfrac{n^3}{n^2+1}\right) = \lim\limits_{n\to\infty} \dfrac{n^2-n^3}{n^3+n^2+n+1}
	=\lim\limits_{n\to\infty} \dfrac{\cancel{n^3}(\frac{1}{n}-1)}{\cancel{n^3}\left(1+\frac{1}{n}+\frac{1}{n^2}+\frac{1}{n^3}\right)}=-1$
\item $\lim\limits_{n\to\infty} \dfrac{(n+1)^4-(n-1)^4}{(n+1)^3+(n-1)^3}=\lim\limits_{n\to\infty} \dfrac{8n^3+8n}{2n^3+6n}
	=\lim\limits_{n\to\infty} \dfrac{\cancel{n^3}(8+8/n^2)}{\cancel{n^3}(2+6/n^2)}=4$
\item $\lim\limits_{n\to\infty} \bigl(\sqrt[\leftroot{0}\uproot{2}3]{n^3+2n^2+1}-n \bigr)=\dfrac{(\sqrt[\leftroot{0}\uproot{2}3]{n^3+2n^2+1}
-n)(\sqrt[\leftroot{0}\uproot{2}3]{(n^3+2n^2+1)^2}+\sqrt[\leftroot{0}\uproot{2}3]{(n^6+2n^5+n^3)}+n^2)}{\sqrt[\leftroot{0}\uproot{2}3]{(n^3+
2n^2+1)^2}+\sqrt[\leftroot{0}\uproot{2}3]{(n^6+2n^5+n^3)}+n^2}=\\
\lim\limits_{n\to\infty} \dfrac{n^3+2n^2+1-n^3}{\sqrt[\leftroot{0}\uproot{2}3]{(n^3+2n^2+1)^2}+
\sqrt[\leftroot{0}\uproot{2}3]{(n^6+2n^5+n^3)}+n^2}=\lim\limits_{n\to\infty}\dfrac{(2+1/n^2)}{\underbrace{(\sqrt[\leftroot{0}\uproot{2}3]{1+\dots}+\sqrt[\leftroot{0}\uproot{2}3]{1+\dots}+1)}_{\text{очев что эта скобра стремится к 3}}}=\dfrac{2}{3}$
\item $\lim\limits_{n\to\infty} \dfrac{\sqrt{n^2+1}-\sqrt{n^2-1}}{\sqrt{n^2+1}-n-1}$
\end{enumerate}

\end{document}
